something

bedrock2/src/bedrock2/Semantics.v
@@ -31,7 +31,8 @@ Section WithIOEvent.
   | qbranch : bool -> qevent
   | qread : access_size -> word -> qevent
   | qwrite : access_size -> word -> qevent
-  | qsalloc : qevent.
+  | qsalloc : qevent
+  | qend: qevent.
 
   Definition q e : qevent :=
     match e with
@@ -200,18 +201,18 @@ Section WithIOEvent.
   Proof. intros H1 H2. induction H1; inversion H2; subst; auto. eapply abs_tr_eq_trans; try eassumption. apply abs_tr_eq_symm. assumption. Qed.
 
   Print abstract_trace.
-  Definition head (a : abstract_trace) : option qevent :=
+  Definition head (a : abstract_trace) : qevent :=
     match a with
-    | empty => None
-    | cons_IO i _ => Some (qIO i)
-    | cons_branch b _ => Some (qbranch b)
-    | cons_read sz a _ => Some (qread sz a)
-    | cons_write sz a _ => Some (qwrite sz a)
-    | cons_salloc _ => Some qsalloc
+    | empty => qend
+    | cons_IO i _ => qIO i
+    | cons_branch b _ => qbranch b
+    | cons_read sz a _ => qread sz a
+    | cons_write sz a _ => qwrite sz a
+    | cons_salloc _ => qsalloc
     end.
   Fixpoint predictor (a(*the whole thing*) : abstract_trace) (t(*so far*) : trace) : option qevent :=
     match a, t with
-    | _, nil => head a
+    | _, nil => Some (head a)
     | cons_IO _ a', cons (IO _) t' => predictor a' t'
     | cons_branch _ a', cons (branch _) t' => predictor a' t'
     | cons_read _ _ a', cons (read _ _) t' => predictor a' t'
@@ -220,26 +221,26 @@ Section WithIOEvent.
     | _, _ => None (*failure*)
     end.
   Search (list ?A -> ?A).
-  Definition option_hd {A : Type} (l : list A) : option A :=
+  Definition nextq (l : list event) : qevent :=
     match l with
-    | a :: _ => Some a
-    | _ => None
+    | a :: _ => q a
+    | nil => qend
     end.
   Definition predicts (f : trace -> option qevent) (t : trace) :=
     forall t1 t2,
       t = t1 ++ t2 ->
-      f t1 = option_map q (option_hd t2).
-  (*Definition sometimes_predicts (f : nat -> trace -> option (option qevent)) (t : trace) :=
-    forall t1 t2,
-      t = t1 ++ t2 ->
-      exists fuel, f fuel t1 = Some (option_map q (option_hd t2)).*)
+      f t1 = Some (nextq t2).
 
   Lemma predictor_works a t :
     generates a t ->
     predicts (predictor a) t.
   Proof.
     intros H. cbv [predicts]. induction H; intros.
-    - simpl. destruct t1, t2; try reflexivity. all: apply app_cons_not_nil in H; destruct H.
+    - destruct t1.
+      + destruct t2.
+        -- reflexivity.
+        -- simpl in H. congruence.
+      + simpl in H. congruence.
     - destruct t1.
       + destruct t2.
         -- simpl in H0. congruence.
